Format lowenheim_formula.v and lowenheim_proof.v

B_Unification/lowenheim_proof.v
@@ -9,689 +9,673 @@ Import ListNotations.
 Import Coq.Init.Tactics.
 Require Export Classical_Prop.
 
-(** *Introduction **)
+(** * Introduction *)
 
-(** In this chapter we provide a proof that our main Lowenheim_Main function defined in lowenheim_formula.v provides a unifier 
-   that is most general. Our final top level proof (found at the end of this file) proves two statements:
-      1) if a term is unifiable, then our own defined Lowenheim_Main function produces a most general unifier (mgu)
-      2) if a term is not unifiable, then our own defined Lownheim_Main function produces a None substitution
-We prove the above statements with a series of proofs and sub-groups of proofs that help us get to the final top-level statements 
-mentioned above.
-**)
+(** In this chapter we provide a proof that our [Lowenheim_Main] function
+    defined in [lowenheim_formula] provides a unifier that is most general. Our
+    final top level proof (found at the end of this file) proves two statements:
+    1) If a term is unifiable, then our own defined [Lowenheim_Main] function
+    produces a most general unifier (mgu). 2) If a term is not unifiable, then
+    our own defined [Lownheim_Main] function produces a [None] substitution. We
+    prove the above statements with a series of proofs and sub-groups of proofs
+    that help us get to the final top-level statements mentioned above. *)
 
-(** * Auxillary declarations and their lemmas useful for the final proofs **)
+(** * Auxillary Declarations and Their Lemmas Useful For the Final Proofs *)
 
-(** In this section we provide definitions and proofs of helper functions, Propositions and lemmas that will be later used
-  in other proofs.
+(** In this section we provide definitions and proofs of helper functions,
+    propositions, and lemmas that will be later used in other proofs. *)
 
-**)
-
-(** This is the definition of an under_term. An under_term is a Proposition, or a relationship between two terms. When a term t is an under_term
-of a term t' then each of the unique variables found within t are also found within the unique variables of t'. 
-**)
+(** This is the definition of an [under_term]. An [under_term] is a proposition,
+    or a relationship between two terms. When a term _t_ is an [under_term] of a
+    term [t'] then each of the unique variables found within _t_ are also found
+    within the unique variables of [t']. *)
 
 Definition under_term (t : term) (t' : term) : Prop :=
   forall (x : var ),
-  (In x (term_unique_vars t) ) -> (In x (term_unique_vars t')) .
+  In x (term_unique_vars t) -> In x (term_unique_vars t').
 
-(** This is a simple lemma for under_terms that states that a term is an under_term of itself. 
-**)
+(** This is a simple lemma for [under_term]s that states that a term is an
+    [under_term] of itself. *)
 
-Lemma under_term_id :
-  forall (t : term),
+Lemma under_term_id : forall (t : term),
   under_term t t.
 Proof.
- intros. firstorder.
+  intros. firstorder.
 Qed.
 
-(** This is a lemma to prove the summation distribution property of the function term_vars: the term_vars of a sum of two_terms
-is equal to the concantentation of the term_vars of each individual term of the original sum.
-**)
+(** This is a lemma to prove the summation distribution property of the function
+    [term_vars]: the [term_vars] of a sum of two terms is equal to the
+    concantentation of the [term_vars] of each individual term of the original
+    sum. *)
 
-Lemma term_vars_distr :
-forall (t1 t2 : term),
- (term_vars (t1 + t2)) = (term_vars t1) ++ (term_vars t2).
+Lemma term_vars_distr : forall (t1 t2 : term),
+  term_vars (t1 + t2) = term_vars t1 ++ term_vars t2.
 Proof.
- intros.
- induction t2.
- - simpl. reflexivity.
- - simpl. reflexivity.
- - simpl. reflexivity.
- - simpl. reflexivity.
- - simpl. reflexivity.
+  intros.
+  induction t2; auto.
 Qed.
 
-(** This is a lemma to prove an intuitive statement: if a variable is within the term_vars (list of variables) of a term, then it is also
-within the term vars of the sum of that term and any other term.
-**)
+(** This is a lemma to prove an intuitive statement: if a variable is within the
+    [term_vars] (list of variables) of a term, then it is also within the
+    [term_vars] of the sum of that term and any other term. *)
 
-Lemma tv_h1:
-forall (t1 t2 : term) ,
-forall (x : var),
- (In x (term_vars t1)) -> (In x (term_vars (t1 + t2))).
+Lemma tv_h1: forall (t1 t2 : term) (x : var),
+  In x (term_vars t1) -> In x (term_vars (t1 + t2)).
 Proof.
-intros. induction t2.
- - simpl. rewrite app_nil_r. apply H.
- - simpl. rewrite app_nil_r. apply H.
- - simpl. pose proof in_or_app as H1. specialize (H1 var (term_vars t1) [v] x). firstorder.
- - rewrite term_vars_distr. apply in_or_app. left. apply H.
- - rewrite term_vars_distr. apply in_or_app. left.  apply H.
+  intros. induction t2.
+  - simpl. rewrite app_nil_r. apply H.
+  - simpl. rewrite app_nil_r. apply H.
+  - simpl. pose proof in_or_app as H1. specialize (H1 var (term_vars t1) [v] x).
+    firstorder.
+  - rewrite term_vars_distr. apply in_or_app. left. apply H.
+  - rewrite term_vars_distr. apply in_or_app. left. apply H.
 Qed.
 
 
-(** This is a lemma similar to the previous one, to prove an intuitive statement: if a variable is within the term_vars (list of variables) of a term, then it is also
-within the term vars of the sum of that term and any other term, but being added from the left side.
-**)
+(** This is a lemma similar to the previous one, to prove an intuitive
+    statement: if a variable is within the [term_vars] (list of variables) of a
+    term, then it is also within the [term_vars] of the sum of that term and any
+    other term, but being added from the left side. *)
 
-Lemma tv_h2:
-forall (t1 t2 : term) ,
-forall (x : var),
- (In x (term_vars t2)) -> (In x (term_vars (t1 + t2))).
+Lemma tv_h2: forall (t1 t2 : term) (x : var),
+  In x (term_vars t2) -> In x (term_vars (t1 + t2)).
 Proof.
-intros. induction t1.
- - simpl. apply H.
- - simpl.  apply H.
- - simpl. pose proof in_or_app as H1. right. apply H. 
- - rewrite term_vars_distr. apply in_or_app. right. apply H.
- - rewrite term_vars_distr. apply in_or_app. right.  apply H.
+  intros. induction t1.
+  - simpl. apply H.
+  - simpl. apply H.
+  - simpl. pose proof in_or_app as H1. right. apply H.
+  - rewrite term_vars_distr. apply in_or_app. right. apply H.
+  - rewrite term_vars_distr. apply in_or_app. right. apply H.
 Qed.
 
 
-(** This is a helper lemma for the under_term relationship : if the sum of two terms is a subterm of another term t', then the left component of the sum is
-   also a subterm of the other term t' 
-   **)
-   
-Lemma helper_2a:
-  forall (t1 t2 t' : term),
+(** This is a helper lemma for the [under_term] relationship : if the sum of two
+    terms is a subterm of another term [t'], then the left component of the sum
+    is also a subterm of the other term [t']. *)
+
+Lemma helper_2a: forall (t1 t2 t' : term),
   under_term (t1 + t2) t' -> under_term t1 t'.
 Proof.
- intros.  unfold under_term in *. intros. specialize (H x).
- pose proof in_dup_and_non_dup as H10. unfold term_unique_vars. unfold term_unique_vars in *.
- pose proof tv_h1 as H7. apply H. specialize (H7 t1 t2 x). specialize (H10 x (term_vars (t1 + t2))). destruct H10 . 
- apply H1. apply H7. pose proof in_dup_and_non_dup as H10. specialize (H10 x (term_vars t1)). destruct H10.
- apply H4.  apply H0. 
-Qed. 
+  intros. unfold under_term in *. intros. specialize (H x).
+  pose proof in_dup_and_non_dup as H10. unfold term_unique_vars.
+  unfold term_unique_vars in *. pose proof tv_h1 as H7. apply H.
+  specialize (H7 t1 t2 x). specialize (H10 x (term_vars (t1 + t2))).
+  destruct H10. apply H1. apply H7. pose proof in_dup_and_non_dup as H10.
+  specialize (H10 x (term_vars t1)). destruct H10. apply H4. apply H0.
+Qed.
 
-  
-(**  This is a helper lemma for the under_term relationship : if the sum of two terms is a subterm of another term t', then the right component of the sum is
-   also a subterm of the other term t' 
-   **)
-   
-Lemma helper_2b:
-  forall (t1 t2 t' : term),
+
+(** This is a helper lemma for the [under_term] relationship : if the sum of two
+    terms is a subterm of another term [t'], then the right component of the sum
+    is also a subterm of the other term [t']. *)
+
+Lemma helper_2b: forall (t1 t2 t' : term),
   under_term (t1 + t2) t' -> under_term t2 t'.
 Proof.
-intros.  unfold under_term in *. intros. specialize (H x). 
-pose proof in_dup_and_non_dup as H10. unfold term_unique_vars. unfold term_unique_vars in *.
- pose proof tv_h2 as H7. apply H. specialize (H7 t1 t2 x). specialize (H10 x (term_vars (t1 + t2))). destruct H10 . 
- apply H1. apply H7. pose proof in_dup_and_non_dup as H10. specialize (H10 x (term_vars t2)). destruct H10.
- apply H4.  apply H0.
-Qed. 
+  intros. unfold under_term in *. intros. specialize (H x).
+  pose proof in_dup_and_non_dup as H10. unfold term_unique_vars.
+  unfold term_unique_vars in *. pose proof tv_h2 as H7. apply H.
+  specialize (H7 t1 t2 x). specialize (H10 x (term_vars (t1 + t2))).
+  destruct H10. apply H1. apply H7. pose proof in_dup_and_non_dup as H10.
+  specialize (H10 x (term_vars t2)). destruct H10. apply H4. apply H0.
+Qed.
 
-(**  This is a helper lemma for lists and their elements : if a variable is a member of a list, then it is equal to the first element 
-of that list or it is a member of the rest of the elements of that list.
-  **)
-  
-Lemma elt_in_list:
- forall (x: var) (a : var) (l : list var),
-  (In x (a::l)) ->
-  x = a \/ (In x l).
+(** This is a helper lemma for lists and their elements: if a variable is a
+    member of a list, then it is equal to the first element of that list or it
+    is a member of the rest of the elements of that list. *)
+
+Lemma elt_in_list: forall (x: var) (a : var) (l : list var),
+  In x (a :: l) ->
+  x = a \/ In x l.
 Proof.
-intros.
-pose proof in_inv as H1.
-specialize (H1 var a x l H).
-destruct H1.
- - left. symmetry in H0. apply H0.
- - right. apply H0.
+  intros.
+  pose proof in_inv as H1.
+  specialize (H1 var a x l H).
+  destruct H1.
+  - left. symmetry in H0. apply H0.
+  - right. apply H0.
 Qed.
 
 
-(**  This is a similar lemma to the previous one, for lists and their elements : if a variable is not a member of a list, then it is not equal to the first element 
-of that list and it is a member of the rest of the elements of that list.
-  **)
-  
-Lemma elt_not_in_list:
- forall (x: var) (a : var) (l : list var),
-  ~ (In x (a::l)) ->
-  x <> a /\ ~ (In x l).
+(** This is a similar lemma to the previous one, for lists and their elements:
+    if a variable is not a member of a list, then it is not equal to the first
+    element of that list and it is not a member of the rest of the elements of
+    that list. *)
+
+Lemma elt_not_in_list: forall (x: var) (a : var) (l : list var),
+  ~ In x (a :: l) ->
+  x <> a /\ ~ In x l.
 Proof.
-intros.
-pose proof not_in_cons. specialize (H0 var x a l). destruct H0.
-specialize (H0 H). apply H0.
+  intros.
+  pose proof not_in_cons. specialize (H0 var x a l). destruct H0.
+  specialize (H0 H). apply H0.
 Qed.
 
-(**  This is a lemma for an intuitive statement for the variables of a term : a variable x belongs to the list of unique variables 
-(term_unique_vars) found within the variable-term that is constructed by variable itself (VAR x).
-  **)
-Lemma in_list_of_var_term_of_var:
-forall (x : var),
+(** This is a lemma for an intuitive statement for the variables of a term: a
+    variable [x] belongs to the list of unique variables ([term_unique_vars])
+    found within the variable-term that is constructed by variable itself
+    [VAR x]. *)
+
+Lemma in_list_of_var_term_of_var: forall (x : var),
   In x (term_unique_vars (VAR x)).
 Proof.
-intros. simpl. left. intuition. 
+  intros. simpl. left. intuition. 
 Qed.
 
 
-
-
-(**  This is a lemma for an intuitive statement for the variables of a term : a variable x belongs to the list of unique variables 
-(term_unique_vars) found within the variable-term that is constructed by variable itself (VAR x).
-  **)
-Lemma var_in_out_list:
-  forall (x : var) (lvar : list var),
-  (In x lvar) \/ ~ (In x lvar).
+Lemma var_in_out_list: forall (x : var) (lvar : list var),
+  In x lvar \/ ~ In x lvar.
 Proof.
- intros.
- pose proof classic as H1. specialize (H1 (In x lvar)). apply H1.
-Qed. 
-
-
-
-
-(** * Proof that Lownheim's algorithm unifes a given term **)
-
-(** In this section, we prove that our own defined lowenheim builder from lowenheim_formula.v (build_lowenheim_subst), produces
-a unifier; that is, given unifiable term and one of unifier of the term, it also produces another unifier of this term (and as explained in 
-terms.v, a unifier is a substitution that when applied to term it produces a term equivalent to the ground term T0.
-**)
-
-
-(** This is a helper lemma for the skeleton function defined on lowenheim_formula.v : If we apply a substitution on a term-variable 
-VAR x , and that substitution is created by the skeleton function build_on_list_of_vars applied on a single input variable x, then the resulting
-term is equivalent to :  the resuting term from applying a substitution on a term-variable 
-VAR x , and that substitution being created by the skeleton function build_on_list_of_vars applied on an input list of variables that contains
-variable x.
-**)
-
-Lemma helper1_easy:
- forall (x: var) (lvar : list var) (sig1 sig2 : subst) (s : term),
- (In x lvar) ->
-  apply_subst (VAR x) (build_on_list_of_vars lvar s sig1 sig2)
-  == 
-  apply_subst (VAR x) (build_on_list_of_vars (cons x nil) s sig1 sig2).
-Proof. 
- intros.
- induction lvar. 
- - simpl. simpl in H. destruct H.
- - apply elt_in_list in H. destruct H.
-  + simpl.  destruct (beq_nat a x) as []eqn:?. 
-   {  apply beq_nat_true in Heqb. destruct (beq_nat x x) as []eqn:?.
-    { rewrite H. reflexivity. }
-    { apply beq_nat_false in Heqb.
-      { destruct Heqb.  }
-      { rewrite Heqb.  apply Heqb0. } }}
-   { simpl in IHlvar. apply IHlvar.  symmetry in H. rewrite H in Heqb. 
-    apply beq_nat_false in Heqb. destruct Heqb. intuition. }
-  + destruct (beq_nat a x) as []eqn:?.
-    { apply beq_nat_true in Heqb.  symmetry in Heqb. rewrite Heqb in IHlvar.  rewrite Heqb.
-        simpl in IHlvar.   simpl. destruct (beq_nat a a) as []eqn:?.
-     {  reflexivity. }
-     { apply IHlvar.  rewrite Heqb in H. apply H. }}
-    { apply beq_nat_false in Heqb. simpl. destruct (beq_nat a x) as []eqn:?.
-     { apply beq_nat_true in Heqb0. rewrite Heqb0 in Heqb.  destruct Heqb. intuition. }
-     { simpl in IHlvar. apply IHlvar.  apply H. }}
-Qed.  
-
-
-
-
-
-(** 
-This is another helper lemma for the skeleton function build_on_list_of_vars and it can be rephrased this way: applying two different substitutions on the same term-variable give the same result. 
-    One subsitution containing only one replacement, and for its own variable. The other subsitution
-    contains the previous replacement but also more replacements for other variables (that are obviously not in the variables
-     of our term-variable). So, the replacements for 
-    the extra variables do not affect the application of the subsitution - hence the resulting term. 
- *)
- 
-Lemma helper_1:
-forall (t' s : term) (v : var) (sig1 sig2 : subst),
-  under_term (VAR v) t' -> 
-  apply_subst (VAR v) (build_on_list_of_vars (term_unique_vars t') s sig1 sig2)
-  == 
-  apply_subst (VAR v) (build_on_list_of_vars (term_unique_vars (VAR v)) s sig1 sig2).
-Proof.
- intros.  unfold under_term in H. specialize (H v). pose proof in_list_of_var_term_of_var as H3.
- specialize (H3 v).  specialize (H H3).  pose proof helper1_easy as H2. 
- specialize (H2 v (term_unique_vars t') sig1 sig2 s).  apply H2. apply H.
+  intros.
+  pose proof classic as H1. specialize (H1 (In x lvar)). apply H1.
 Qed.
 
 
+(** * Proof That Lownheim's Algorithm Unifies a Given Term *)
 
+(** In this section, we prove that our own defined Lowenheim builder from
+    [lowenheim_formula] ([build_lowenheim_subst]), produces a unifier; that is,
+    given unifiable term and one unifier of the term, it also produces another
+    unifier of this term (and as explained in the [terms] library, a unifier is
+    a substitution that when applied to term it produces a term equivalent to
+    the ground term [T0]. *)
 
+(** This is a helper lemma for the skeleton function defined in
+    [lowenheim_formula]: If we apply a substitution on a term-variable [VAR x],
+    and that substitution is created by the skeleton function
+    [build_on_list_of_vars] applied on a single input variable [x], then the
+    resulting term is equivalent to: the resuting term from applying a
+    substitution on a term-variable [VAR x], and that substitution being created
+    by the skeleton function [build_on_list_of_vars] applied on an input list of
+    variables that contains variable [x]. *)
 
-
-(**
-Lemma 10.4.5 from book X on page 254-255 . 
-This a very significant lemma used later for the proof that our lownheim builder function (not the Main function, but the 
-builder function), gives a unifier (not necessarily an mgu, which would be a next step of the proof). 
-It states that if a term t is an under_term of another term t' , then applying a substitution - a substitution created by the giving the list of
-variables of term t' on the skeleton function build_list_of_vars -, on the term t, a term that has the same format : 
-(s + T1) * sig1(t) + s*sig2(t) as the each replacements of each variable on any ubsistution created 
-by skeleton function : (s + T1) * sig1(x) + s*sig2(x) .
-*)
-
-Lemma subs_distr_vars_ver2 :
-  forall (t t' : term) (s : term) (sig1 sig2 : subst),
-  (under_term t t') ->
-  apply_subst t (build_on_list_of_vars  (term_unique_vars t') s sig1 sig2)
-    ==
-  (s + T1) * (apply_subst t sig1) + s * (apply_subst t sig2).
+Lemma helper1_easy: forall (x: var) (lvar : list var)
+                           (sig1 sig2 : subst) (s : term),
+  In x lvar ->
+  apply_subst (VAR x) (build_on_list_of_vars lvar s sig1 sig2) ==
+  apply_subst (VAR x) (build_on_list_of_vars [x] s sig1 sig2).
 Proof.
- intros. generalize dependent t'.  induction t.
+  intros.
+  induction lvar.
+  - simpl. simpl in H. destruct H.
+  - apply elt_in_list in H. destruct H.
+    + simpl. destruct (beq_nat a x) as []eqn:?.
+      * apply beq_nat_true in Heqb. destruct (beq_nat x x) as []eqn:?.
+        -- rewrite H. reflexivity.
+        -- apply beq_nat_false in Heqb.
+           ++ destruct Heqb.
+           ++ rewrite Heqb. apply Heqb0.
+      * simpl in IHlvar. apply IHlvar. symmetry in H. rewrite H in Heqb.
+        apply beq_nat_false in Heqb. destruct Heqb. intuition.
+    + destruct (beq_nat a x) as []eqn:?.
+      * apply beq_nat_true in Heqb. symmetry in Heqb. rewrite Heqb in IHlvar.
+        rewrite Heqb. simpl in IHlvar. simpl. destruct (beq_nat a a) as []eqn:?.
+        -- reflexivity.
+        -- apply IHlvar. rewrite Heqb in H. apply H.
+      * apply beq_nat_false in Heqb. simpl. destruct (beq_nat a x) as []eqn:?.
+        -- apply beq_nat_true in Heqb0. rewrite Heqb0 in Heqb. destruct Heqb.
+           intuition.
+        -- simpl in IHlvar. apply IHlvar. apply H.
+Qed.
+
+
+(** This is another helper lemma for the skeleton function
+    [build_on_list_of_vars] and it can be rephrased this way: applying two
+    different substitutions on the same term-variable give the same result. One
+    subsitution containing only one replacement, and for its own variable. The
+    other subsitution contains the previous replacement but also more
+    replacements for other variables (that are obviously not in the variables of
+    our term-variable). So, the replacements for the extra variables do not
+    affect the application of the subsitution - hence the resulting term. *)
+
+Lemma helper_1: forall (t' s : term) (v : var) (sig1 sig2 : subst),
+  under_term (VAR v) t' ->
+  apply_subst (VAR v)
+              (build_on_list_of_vars (term_unique_vars t') s sig1 sig2) ==
+  apply_subst (VAR v)
+              (build_on_list_of_vars (term_unique_vars (VAR v)) s sig1 sig2).
+Proof.
+  intros. unfold under_term in H. specialize (H v).
+  pose proof in_list_of_var_term_of_var as H3. specialize (H3 v).
+  specialize (H H3). pose proof helper1_easy as H2.
+  specialize (H2 v (term_unique_vars t') sig1 sig2 s). apply H2. apply H.
+Qed.
+
+
+(** Lemma 10.4.5 from book X on page 254-255. This a very significant lemma used
+    later for the proof that our Lownheim builder function (not the Main
+    function, but the builder function), gives a unifier (not necessarily an
+    mgu, which would be a next step of the proof). It states that if a term _t_
+    is an [under_term] of another term [t'], then applying a substitution--a
+    substitution created by giving the list of variables of term [t'] on the
+    skeleton function [build_list_of_vars]--, on the term _t_, a term that has
+    the same format: $(s + 1) \ast \sigma_{1}(t) + s \ast \sigma_{2}(t)$ as the
+    each replacements of each variable on any substitution created by skeleton
+    function: $(s + 1) \ast \sigma_{1}(x) + s \ast \sigma_{2}(x)$. *)
+
+Lemma subs_distr_vars_ver2 : forall (t t' s : term) (sig1 sig2 : subst),
+  under_term t t' ->
+  apply_subst t (build_on_list_of_vars (term_unique_vars t') s sig1 sig2) ==
+  (s + T1) * apply_subst t sig1 + s * apply_subst t sig2.
+Proof.
+  intros. generalize dependent t'. induction t.
   - intros t'. repeat rewrite ground_term_cannot_subst.
-    + rewrite mul_comm with (x := s + T1). rewrite distr. repeat rewrite mul_T0_x. rewrite mul_comm with (x := s).
-      rewrite mul_T0_x.  repeat rewrite sum_x_x. reflexivity.
+    + rewrite mul_comm with (x := s + T1). rewrite distr.
+      repeat rewrite mul_T0_x. rewrite mul_comm with (x := s).
+      rewrite mul_T0_x. repeat rewrite sum_x_x. reflexivity.
     + unfold ground_term. reflexivity.
     + unfold ground_term. reflexivity.
     + unfold ground_term. reflexivity.
   - intros t'. repeat rewrite ground_term_cannot_subst.
-    + rewrite mul_comm with (x := s + T1). rewrite mul_id. rewrite mul_comm with (x := s). rewrite mul_id. rewrite sum_comm with (x := s).
-      repeat rewrite sum_assoc. rewrite sum_x_x.  rewrite sum_comm with (x := T1). rewrite sum_id. reflexivity.
-    +  unfold ground_term. reflexivity.
-    +  unfold ground_term. reflexivity.
+    + rewrite mul_comm with (x := s + T1). rewrite mul_id.
+      rewrite mul_comm with (x := s). rewrite mul_id.
+      rewrite sum_comm with (x := s).
+      repeat rewrite sum_assoc. rewrite sum_x_x.
+      rewrite sum_comm with (x := T1). rewrite sum_id. reflexivity.
     + unfold ground_term. reflexivity.
-  - intros. rewrite helper_1 .
-    + unfold term_unique_vars. unfold term_vars. unfold var_set_create_unique. unfold var_set_includes_var. unfold build_on_list_of_vars.
-    rewrite var_subst. reflexivity. 
-    + apply H. 
-  -  intros. specialize (IHt1 t'). specialize (IHt2 t').  repeat rewrite subst_sum_distr_opp. 
-      rewrite IHt1. rewrite IHt2.
-    + rewrite distr. rewrite distr. repeat rewrite sum_assoc. rewrite sum_comm with (x := (s + T1) * apply_subst t2 sig1)
-      (y := (s * apply_subst t1 sig2 + s * apply_subst t2 sig2)). repeat rewrite sum_assoc.
-      rewrite sum_comm with (x := s * apply_subst t2 sig2 ) (y := (s + T1) * apply_subst t2 sig1).
+    + unfold ground_term. reflexivity.
+    + unfold ground_term. reflexivity.
+  - intros. rewrite helper_1.
+    + unfold term_unique_vars. unfold term_vars. unfold var_set_create_unique.
+      unfold var_set_includes_var. unfold build_on_list_of_vars.
+      rewrite var_subst. reflexivity.
+    + apply H.
+  - intros. specialize (IHt1 t'). specialize (IHt2 t').
+    repeat rewrite subst_sum_distr_opp. rewrite IHt1. rewrite IHt2.
+    + rewrite distr. rewrite distr. repeat rewrite sum_assoc.
+      rewrite sum_comm with (x := (s + T1) * apply_subst t2 sig1)
+        (y := s * apply_subst t1 sig2 + s * apply_subst t2 sig2).
+      repeat rewrite sum_assoc.
+      rewrite sum_comm with (x := s * apply_subst t2 sig2)
+        (y := (s + T1) * apply_subst t2 sig1).
       repeat rewrite sum_assoc. reflexivity.
-    + pose helper_2b as H2. specialize (H2 t1 t2 t'). apply H2. apply H. 
-    + pose helper_2a as H2. specialize (H2 t1 t2 t'). apply H2. apply H. 
-  - intros. specialize (IHt1 t'). specialize (IHt2 t'). repeat rewrite subst_mul_distr_opp. rewrite IHt1. rewrite IHt2.
-    + rewrite distr. rewrite mul_comm with (y := ((s + T1) * apply_subst t2 sig1)).
-    rewrite distr. rewrite mul_comm with (y := (s * apply_subst t2 sig2)). rewrite distr.
-    repeat rewrite mul_assoc. repeat rewrite mul_comm with (x := apply_subst t2 sig1).
-    repeat rewrite mul_assoc.
-    rewrite mul_assoc_opp with (x := (s + T1)) (y := (s + T1)) . rewrite mul_x_x.
-    rewrite mul_assoc_opp with (x := (s + T1)) (y := s). rewrite mul_comm with (x := (s + T1)) (y := s).
-    rewrite distr. rewrite mul_x_x. rewrite mul_id_sym. rewrite sum_x_x. rewrite mul_T0_x.
-    repeat rewrite mul_assoc. rewrite mul_comm with (x := apply_subst t2 sig2 ).
-    repeat rewrite mul_assoc. rewrite mul_assoc_opp with (x := s ) (y := (s + T1)).
-    rewrite distr. rewrite mul_x_x. rewrite mul_id_sym. rewrite sum_x_x. rewrite mul_T0_x.
-    repeat rewrite sum_assoc. rewrite sum_assoc_opp with (x := T0) (y := T0). rewrite sum_x_x. rewrite sum_id.
-    repeat rewrite mul_assoc. rewrite mul_comm with (x := apply_subst t2 sig2) (y := s * apply_subst t1 sig2).
-    repeat rewrite mul_assoc. rewrite mul_assoc_opp with (x := s). rewrite mul_x_x. reflexivity.
-    + pose helper_2b as H2. specialize (H2 t1 t2 t'). apply H2. apply H. 
-    + pose helper_2a as H2. specialize (H2 t1 t2 t'). apply H2. apply H. 
+    + pose helper_2b as H2. specialize (H2 t1 t2 t'). apply H2. apply H.
+    + pose helper_2a as H2. specialize (H2 t1 t2 t'). apply H2. apply H.
+  - intros. specialize (IHt1 t'). specialize (IHt2 t').
+    repeat rewrite subst_mul_distr_opp. rewrite IHt1. rewrite IHt2.
+    + rewrite distr.
+      rewrite mul_comm with (y := (s + T1) * apply_subst t2 sig1).
+      rewrite distr. rewrite mul_comm with (y := s * apply_subst t2 sig2).
+      rewrite distr. repeat rewrite mul_assoc.
+      repeat rewrite mul_comm with (x := apply_subst t2 sig1).
+      repeat rewrite mul_assoc.
+      rewrite mul_assoc_opp with (x := s + T1) (y := s + T1). rewrite mul_x_x.
+      rewrite mul_assoc_opp with (x := s + T1) (y := s).
+      rewrite mul_comm with (x := s + T1) (y := s). rewrite distr.
+      rewrite mul_x_x. rewrite mul_id_sym. rewrite sum_x_x. rewrite mul_T0_x.
+      repeat rewrite mul_assoc.
+      rewrite mul_comm with (x := apply_subst t2 sig2).
+      repeat rewrite mul_assoc.
+      rewrite mul_assoc_opp with (x := s) (y := s + T1). rewrite distr.
+      rewrite mul_x_x. rewrite mul_id_sym. rewrite sum_x_x. rewrite mul_T0_x.
+      repeat rewrite sum_assoc. rewrite sum_assoc_opp with (x := T0) (y := T0).
+      rewrite sum_x_x. rewrite sum_id. repeat rewrite mul_assoc.
+      rewrite mul_comm with (x := apply_subst t2 sig2)
+        (y := s * apply_subst t1 sig2).
+      repeat rewrite mul_assoc. rewrite mul_assoc_opp with (x := s).
+      rewrite mul_x_x. reflexivity.
+    + pose helper_2b as H2. specialize (H2 t1 t2 t'). apply H2. apply H.
+    + pose helper_2a as H2. specialize (H2 t1 t2 t'). apply H2. apply H.
 Qed.
 
 
+(** This is an intermediate lemma occuring by the previous lemma 10.4.5.
+    Utilizing lemma 10.4.5 and also using two substitutions for the skeleton
+    function [build_on_list_vars] gives a substituion the unifies the term; the
+    two substitutions being a known unifier of the term and the identity
+    substitution. *)
 
-(**
-This is an intermediate lemma occuring by the previous lemma 10.4.5 .
-Utilizing lemma 10.4.5 and also using two sigmas for the skeleton function build_on_list_vars
-gives a substituion the unifies the term; the two sigmas being a known unifier of the term and the identity 
-substitution.
-*)
-
-Lemma specific_sigmas_unify:
-  forall (t : term) (tau : subst),
-  (unifier t tau) -> 
-  (apply_subst t (build_on_list_of_vars  (term_unique_vars t) t (build_id_subst (term_unique_vars t)) tau )
-  ) == T0 .
-  Proof.
-  intros. 
+Lemma specific_sigmas_unify: forall (t : term) (tau : subst),
+  unifier t tau ->
+  apply_subst t (build_on_list_of_vars
+                  (term_unique_vars t) t (build_id_subst (term_unique_vars t))
+                  tau) ==
+  T0.
+Proof.
+  intros.
   rewrite subs_distr_vars_ver2.
-  - rewrite id_subst. rewrite mul_comm with (x := t + T1). rewrite distr. rewrite mul_x_x. rewrite mul_id_sym. rewrite sum_x_x.
-    rewrite sum_id. 
+  - rewrite id_subst. rewrite mul_comm with (x := t + T1). rewrite distr.
+    rewrite mul_x_x. rewrite mul_id_sym. rewrite sum_x_x. rewrite sum_id.
     unfold unifier in H. rewrite H. rewrite mul_T0_x_sym. reflexivity.
-  -  apply under_term_id.
+  - apply under_term_id.
 Qed.
 
-(** This is the resulting lemma from this sub-section :
-Our lowenheim's subsitution builder produces a unifier for an input term; namely, a substitution that 
-unifies the term, given that term is unifiable and we know an already existing unifier tau. 
-*)
+(** This is the resulting lemma from this subsection: Our Lowenheim's
+    subsitution builder produces a unifier for an input term; namely, a
+    substitution that unifies the term, given that term is unifiable and we know
+    an already existing unifier $\tau$. *)
 
-Lemma lownheim_unifies:
-  forall (t : term) (tau : subst),
-  (unifier t tau) -> 
-  (apply_subst t (build_lowenheim_subst t tau)) == T0.
+Lemma lownheim_unifies: forall (t : term) (tau : subst),
+  unifier t tau ->
+  apply_subst t (build_lowenheim_subst t tau) == T0.
 Proof.
-intros. unfold build_lowenheim_subst. apply specific_sigmas_unify. apply H.
+  intros. unfold build_lowenheim_subst. apply specific_sigmas_unify. apply H.
 Qed.
 
 
 
-(** * Proof that Lownheim's algorithm produces a most general unifier **)
+(** * Proof That Lownheim's algorithm Produces a Most General Unifier *)
 
-(** In the previous section we proved that our lowenheim builder produces a unifier, if we already know an existing unifier
-of the term. In this sub-section we prove that that unifier is a most general unifier. 
-**)
-
-
-(**  **Proof that Lownheim's algorithm produces a reproductive unifier **)
-
-(**
-In this sub-section we will prove that our lowenheim builder gives a unifier that is reproductive; this will help us in the proof
-that the resulting unifier is an mgu, since a reproductive unifier is a "stronger" property than an mgu.
-
-**)
+(** In the previous section we proved that our Lowenheim builder produces a
+    unifier, if we already know an existing unifier of the term. In this
+    section we prove that that unifier is a most general unifier. *)
 
 
-(** This is a lemma for an intuitive statement for the skeleton function build_on_list_vars : if a variable x is in a list l, and we
-apply a substitution created by the build_on_list_vars function given input list l, on the term-variable VAR x, then we get the replacement
-for that particular variable that was contained in the original substitution. So basically if build_on_list_of_vars is applied on a list
-of variables l (x1,x2,x3...xn), then the resulting substitution is in the format [(x1, (s + T1) * sig1(x1) + s*sig2(x1)),. , .] for each
-xi. If we apply that substitution on the term-variable x1, we will get the initial format of the replacement : (s + T1) * sig1(x1) + s*sig2(x1)).
-It can be thought as "reverse application" of the skeleton function.
-**)
+(** ** Proof That Lownheim's algorithm produces a reproductive unifier *)
 
-Lemma lowenheim_rephrase1_easy :
-  forall (l : list var) (x : var) (sig1 : subst) (sig2 : subst) (s : term),
-  (In x l) -> 
-  (apply_subst (VAR x) (build_on_list_of_vars l s  sig1 sig2)) == 
-  (s + T1) * (apply_subst (VAR x) sig1 )  + s * (apply_subst (VAR x) sig2 ).
+(** In this subsection we will prove that our Lowenheim builder gives a
+    unifier that is reproductive; this will help us in the proof that the
+    resulting unifier is an mgu, since a reproductive unifier is a "stronger"
+    property than an mgu. *)
+
+
+(** This is a lemma for an intuitive statement for the skeleton function
+    [build_on_list_vars]: if a variable [x] is in a list [l], and we apply a
+    substitution created by the [build_on_list_vars] function given input list
+    [l], on the term-variable [VAR x], then we get the replacement for that
+    particular variable that was contained in the original substitution. So
+    basically if [build_on_list_of_vars] is applied on a list of variables [l]
+    ($x_{1}, x{2}, x_{3}, ..., x_{n}$), then the resulting substitution is in
+    the format
+    $x_{i} \mapsto (s + 1) \ast \sigma_{1}(x_{i}) + s \ast \sigma_{2}(x_{i})$
+    for each $x_{i}$. If we apply that substitution on the term-variable $x_{1},
+    we will get the initial format of the replacement:
+    $(s + 1) \ast \sigma_{1}(x_{1}) + s \ast \sigma_{2}(x_{1})$. It can be
+    thought as "reverse application" of the skeleton function. *)
+
+Lemma lowenheim_rephrase1_easy : forall (l : list var) (x : var)
+                                        (sig1 sig2 : subst) (s : term),
+  In x l ->
+  apply_subst (VAR x) (build_on_list_of_vars l s  sig1 sig2) ==
+  (s + T1) * apply_subst (VAR x) sig1  + s * apply_subst (VAR x) sig2.
 Proof.
-intros.
-induction l.
-- simpl. unfold In in H. destruct H.
--  apply elt_in_list in H. destruct H.
-  + simpl. destruct (beq_nat a x) as []eqn:?. 
-    { rewrite H.  reflexivity. }
-    { pose proof beq_nat_false as H2. specialize (H2 a x).
-      specialize (H2 Heqb). intuition. symmetry in H. specialize (H2 H).  inversion H2. }
-  + simpl. destruct (beq_nat a x) as []eqn:?. 
-    { symmetry in Heqb.  pose proof beq_nat_eq  as H2. specialize (H2 a x). specialize (H2 Heqb). rewrite H2.
-      reflexivity. }
-    { apply IHl. apply H. }
+  intros.
+  induction l.
+  - simpl. unfold In in H. destruct H.
+  - apply elt_in_list in H. destruct H.
+    + simpl. destruct (beq_nat a x) as []eqn:?.
+      * rewrite H.  reflexivity.
+      * pose proof beq_nat_false as H2. specialize (H2 a x).
+        specialize (H2 Heqb). intuition. symmetry in H. specialize (H2 H).
+        inversion H2.
+    + simpl. destruct (beq_nat a x) as []eqn:?.
+      * symmetry in Heqb. pose proof beq_nat_eq as H2. specialize (H2 a x).
+        specialize (H2 Heqb). rewrite H2. reflexivity.
+      * apply IHl. apply H.
 Qed.
 
 
+(** This is a helper lemma for an intuitive statement: if a variable [x] is
+    found in a list of variables [l], then applying the subsitution created by
+    the [build_id_subst] function given input list [l], on the term-variable
+    [VAR x], we will get the same [VAR x] back. *)
 
-(** This is a helper lemma for an intuitive statement : if a variable x is found on a list of variables l, then applying the subsitution
-created by the build_id_subst function given input list l, on the term-variable VAR x, we will get the same VAR x back. 
-**)
-
-Lemma helper_3a:
-forall (x: var) (l: list var),
-In x l -> 
+Lemma helper_3a: forall (x: var) (l: list var),
+  In x l ->
   apply_subst (VAR x) (build_id_subst l) == VAR x.
 Proof.
-intros. induction l.
- -  unfold build_id_subst. simpl. reflexivity.
- -  apply elt_in_list in H. destruct H.
-   + simpl. destruct (beq_nat a x) as []eqn:?.
-    { rewrite H. reflexivity. }
-    {  pose proof beq_nat_false as H2. specialize (H2 a x).
-       specialize (H2 Heqb). intuition. symmetry in H. specialize (H2 H).  inversion H2. }
-   + simpl.  destruct (beq_nat a x) as []eqn:?. 
-    { symmetry in Heqb.  pose proof beq_nat_eq  as H2. specialize (H2 a x). specialize (H2 Heqb). rewrite H2.
-      reflexivity. }
-    {  apply IHl. apply H. }
-Qed.
-    
-
-
-(** 
-This is a lemma for an intuitive statement for the lowenheim builder,very similar to lemma lowenheim_rephrase1_easy : 
- applying lowenheim's subtitution given an input term t,on any term-variable of the term t, gives us the initial format 
-  of the replacement for that variable (lowenheim's reverse application ) 
-  *)
-  
-Lemma lowenheim_rephrase1 :
-  forall (t : term) (tau : subst) (x : var),
-  (unifier t tau) -> 
-  (In x (term_unique_vars t)) -> 
-  (apply_subst (VAR x) (build_lowenheim_subst t tau)) == 
-  (t + T1) * (VAR x) + t * (apply_subst (VAR x) tau).
-  Proof.
- intros. 
-  unfold build_lowenheim_subst. pose proof lowenheim_rephrase1_easy as H1. 
-  specialize (H1 (term_unique_vars t) x (build_id_subst (term_unique_vars t)) tau t).
-  rewrite helper_3a in H1. 
- - apply H1. apply H0.
- -  apply H0.
+  intros. induction l.
+  - unfold build_id_subst. simpl. reflexivity.
+  - apply elt_in_list in H. destruct H.
+    + simpl. destruct (beq_nat a x) as []eqn:?.
+      * rewrite H. reflexivity.
+      * pose proof beq_nat_false as H2. specialize (H2 a x).
+        specialize (H2 Heqb). intuition. symmetry in H. specialize (H2 H).
+        inversion H2.
+    + simpl. destruct (beq_nat a x) as []eqn:?.
+      * symmetry in Heqb.  pose proof beq_nat_eq as H2. specialize (H2 a x).
+        specialize (H2 Heqb). rewrite H2. reflexivity.
+      * apply IHl. apply H.
 Qed.
 
 
+(** This is a lemma for an intuitive statement for the Lowenheim builder,
+    very similar to lemma [lowenheim_rephrase1_easy]: applying Lowenheim's
+    subtitution given an input term _t_, on any term-variable of the term _t_,
+    gives us the initial format of the replacement for that variable
+    (Lowenheim's reverse application). *)
 
-
-(**
-This is a lemma for an intuitive statement for the skeleton function build_on_list_vars tha resemebles a lot 
-lowenheim_rephrase1_easy : 
-if a variable x is not in a list l, and we
-apply a substitution created by the build_on_list_vars function given input list l, on the term-variable VAR x, 
-then we get the term-variable VAR xback; that is expected since the replacements in the substitution should not contain
-any entry with variable x.
-*)
-
-Lemma lowenheim_rephrase2_easy :
-  forall (l : list var) (x : var) (sig1 : subst) (sig2 : subst) (s : term),
-  ~ (In x l) -> 
-  (apply_subst (VAR x) (build_on_list_of_vars l s  sig1 sig2)) == 
-  (VAR x).
+Lemma lowenheim_rephrase1 : forall (t : term) (tau : subst) (x : var),
+  unifier t tau ->
+  In x (term_unique_vars t) ->
+  apply_subst (VAR x) (build_lowenheim_subst t tau) ==
+  (t + T1) * (VAR x) + t * apply_subst (VAR x) tau.
 Proof.
-intros. unfold not in H. 
-induction  l.
--  simpl. reflexivity.
-- simpl. pose proof elt_not_in_list as H2. specialize (H2 x a l). unfold not in H2.
-  specialize (H2 H). destruct H2. 
-  destruct (beq_nat a x) as []eqn:?. 
-  + symmetry in Heqb. apply beq_nat_eq in Heqb. symmetry in Heqb.  specialize (H0 Heqb).  destruct H0.
-  + simpl in IHl. apply IHl.  apply H1.
-Qed. 
-
-
-
-(** This is a lemma for an intuitive statement for the lowenheim builder,very similar to lemma lowenheim_rephrase2_easy
- and lowenheim_rephrase1: 
- applying lowenheim's subtitution given an input term t, on any term-variable not of the ones of term t, gives us back 
-  the same term-variable.
-  *)
-
-Lemma lowenheim_rephrase2 :
-  forall (t : term) (tau : subst) (x : var),
-  (unifier t tau) -> 
-  ~ (In x (term_unique_vars t)) -> 
-  (apply_subst (VAR x) (build_lowenheim_subst t tau)) == 
-  (VAR x).
-Proof.
-intros. unfold build_lowenheim_subst.  pose proof lowenheim_rephrase2_easy as H2. 
-specialize (H2 (term_unique_vars t) x (build_id_subst (term_unique_vars t)) tau t).
-specialize (H2 H0). apply H2.  
-Qed.
-
-  
-
-
-(** This is the resulting lemma of the sector: our lowenheim builder build_lownheim_subst gives a reproductive unifier 
-*)
-
-Lemma lowenheim_reproductive:
-  forall (t : term) (tau : subst),
-  (unifier t tau) -> 
-  reproductive_unifier t (build_lowenheim_subst t tau) .
-Proof.
- intros. unfold reproductive_unifier. intros. 
-  pose proof var_in_out_list. specialize (H2 x (term_unique_vars t)). destruct H2.
-  {
-  rewrite lowenheim_rephrase1.
-  - rewrite subst_sum_distr_opp. rewrite subst_mul_distr_opp. rewrite subst_mul_distr_opp.
-    unfold unifier in H1. rewrite H1. rewrite mul_T0_x. rewrite subst_sum_distr_opp.
-    rewrite H1. rewrite ground_term_cannot_subst.
-    + rewrite sum_id. rewrite mul_id. rewrite sum_comm. rewrite sum_id. reflexivity.
-    + unfold ground_term. intuition.
-  - apply H.  
-  - apply H2. 
-  }
-  { rewrite lowenheim_rephrase2.
-    - reflexivity.
-    - apply H.
-    -  apply H2.
-  }
+  intros.
+  unfold build_lowenheim_subst. pose proof lowenheim_rephrase1_easy as H1.
+  specialize (H1 (term_unique_vars t) x
+    (build_id_subst (term_unique_vars t)) tau t).
+  rewrite helper_3a in H1.
+  - apply H1. apply H0.
+  - apply H0.
 Qed.
 
 
+(** This is a lemma for an intuitive statement for the skeleton function
+    [build_on_list_vars] that resemebles a lot of [lowenheim_rephrase1_easy]: if
+    a variable [x] is not in a list [l], and we apply a substitution created by
+    the [build_on_list_vars] function given input list [l], on the term-variable
+    [VAR x], then we get the term-variable [VAR x] back; that is expected since
+    the replacements in the substitution should not contain any entry with
+    variable [x]. *)
 
-
-(**  **Proof that Lowenheim's algorithm (our lowenheim builder) produces a most general unifier **)
-
-(**
-In this sub-section we will prove that our lowenheim builder gives a unifier that is most general; this will help us a lot in the top-level
-proof that the Main_Lownheim function gives an mgu.
-
-**)
-
-
-(** Here is the sub-section's resulting lemma. Given a unifiable term t, a unifier of t, then our lowenheim builder
-(build_lownheim_subst) gives a most general unifier (mgu) .
-**)
-
-Lemma lowenheim_most_general_unifier:
-  forall (t : term) (tau : subst),
-  (unifier t tau) -> 
-  most_general_unifier t (build_lowenheim_subst t tau) .
+Lemma lowenheim_rephrase2_easy : forall (l : list var) (x : var)
+                                        (sig1 sig2 : subst) (s : term),
+  ~ (In x l) ->
+  apply_subst (VAR x) (build_on_list_of_vars l s sig1 sig2) ==
+  VAR x.
 Proof.
-intros. apply reproductive_is_mgu. apply lowenheim_reproductive.  apply H.
+  intros. unfold not in H.
+  induction l.
+  - simpl. reflexivity.
+  - simpl. pose proof elt_not_in_list as H2. specialize (H2 x a l).
+    unfold not in H2. specialize (H2 H). destruct H2.
+    destruct (beq_nat a x) as []eqn:?.
+    + symmetry in Heqb. apply beq_nat_eq in Heqb. symmetry in Heqb.
+      specialize (H0 Heqb). destruct H0.
+    + simpl in IHl. apply IHl. apply H1.
+Qed.
+
+
+(** This is a lemma for an intuitive statement for the Lowenheim builder,
+    very similar to lemma [lowenheim_rephrase2_easy] and [lowenheim_rephrase1]:
+    applying Lowenheim's subtitution given an input term _t_, on any
+    term-variable not of the ones of term _t_, gives us back the same
+    term-variable. *)
+
+Lemma lowenheim_rephrase2 : forall (t : term) (tau : subst) (x : var),
+  unifier t tau ->
+  ~ (In x (term_unique_vars t)) ->
+  apply_subst (VAR x) (build_lowenheim_subst t tau) ==
+  VAR x.
+Proof.
+  intros. unfold build_lowenheim_subst.
+  pose proof lowenheim_rephrase2_easy as H2.
+  specialize (H2 (term_unique_vars t) x
+    (build_id_subst (term_unique_vars t)) tau t).
+  specialize (H2 H0). apply H2.
+Qed.
+
+
+(** This is the resulting lemma of the secton: our Lowenheim builder
+    [build_lownheim_subst] gives a reproductive unifier. *)
+
+Lemma lowenheim_reproductive: forall (t : term) (tau : subst),
+  unifier t tau ->
+  reproductive_unifier t (build_lowenheim_subst t tau).
+Proof.
+  intros. unfold reproductive_unifier. intros.
+  pose proof var_in_out_list. specialize (H2 x (term_unique_vars t)).
+  destruct H2.
+  - rewrite lowenheim_rephrase1.
+    + rewrite subst_sum_distr_opp. rewrite subst_mul_distr_opp.
+      rewrite subst_mul_distr_opp. unfold unifier in H1. rewrite H1.
+      rewrite mul_T0_x. rewrite subst_sum_distr_opp. rewrite H1.
+      rewrite ground_term_cannot_subst.
+      * rewrite sum_id. rewrite mul_id. rewrite sum_comm. rewrite sum_id.
+        reflexivity.
+      * unfold ground_term. intuition.
+    + apply H.
+    + apply H2.
+  - rewrite lowenheim_rephrase2.
+    + reflexivity.
+    + apply H.
+    + apply H2.
+Qed.
+
+
+(** ** Proof That Lowenheim's Algorithm Produces a Most General Unifier *)
+
+(** In this subsection we will prove that our Lowenheim builder gives a
+    unifier that is most general; this will help us a lot in the top-level proof
+    that the [Main_Lownheim] function gives an mgu. *)
+
+(** Here is the subsection's resulting lemma. Given a unifiable term _t_, a
+    unifier of _t_, then our Lowenheim builder ([build_lownheim_subst])
+    gives a most general unifier (mgu). *)
+
+Lemma lowenheim_most_general_unifier: forall (t : term) (tau : subst),
+  unifier t tau ->
+  most_general_unifier t (build_lowenheim_subst t tau).
+Proof.
+  intros. apply reproductive_is_mgu. apply lowenheim_reproductive. apply H.
 Qed.
 
 
 
+(** * Proof of Correctness of Our Main Lowenheim Function -
+      [Lowenheim_Main] *)
 
-
-(** * Proof of correctness of our main lowenheim function - Lowenheim_Main *)
-
-(** In this section we prove that our own defined Lownheim function satisfies its two main requirements:
-      1) if a term is unifiable, then Lowenheim_Main function produces a most general unifier (mgu).
-      2) if a term is not unifiable, then Lownheim_Main function produces a None substitution.
-  The final top-level proofs is at the end of this section. To get there, we prove a series of intermediate lemmas that are needed for the 
-  final proof.
-
-**)
+(** In this section we prove that our own defined Lownheim function
+    satisfies its two main requirements: 1) If a term is unifiable, then
+    [Lowenheim_Main] function produces a most general unifier (mgu). 2) If a
+    term is not unifiable, then Lownheim_Main function produces a [None]
+    substitution. The final top-level proof is at the end of this section. To
+    get there, we prove a series of intermediate lemmas that are needed for the
+    final proof. *)
 
 
 (** ** Utilities *)
 
+(** In this section we provide helper "utility" lemmas and functions that are
+    used in the proofs of intermediate lemmas that are in turn used in the final
+    proof. *)
 
-(** In this section we provide helper "utility" helper lemmas and functions that are used in the proofs of intermediate lemmas
-that are in turn used in the final proof.
-
-**)
-
-(** This is a function that converts a subst option (substitution option) to a subst (substitution). It is designed to be used mainly
-for subst options that are "Some subst". If the input subst option is not "Some" and is "None" then the return type is the 
-nil substitution, but that case should not normally be considered. This function is useful because many functions and lemmas are defined
-for the substitution type not the option substitution type (option subst).
-**)
+(** This is a function that converts a [option subst] to a [subst]. It is
+    designed to be used mainly for [option subst]s that are $Some \sigma$. If
+    the input [option subst] is not [Some] and is [None] then it returns the
+    [nil] substitution, but that case should not normally be considered. This
+    function is useful because many functions and lemmas are defined for the
+    substitution type not the option substitution type. *)
 
 Definition convert_to_subst (so : option subst) : subst :=
   match so with
   | Some s => s
-  | None => nil (* normally not considered *)
+  | None => [] (* normally not considered *)
   end.
 
 
+(** This is an intuitive helper lemma that proves that if an empty substitution
+    is applied on any term _t_, then the resulting term is the same input term
+    _t_. *)
 
-(** This is an intuitive helper lemma that proves that if an empty substitution is applied on any term t, then the resulting term
-is the same input term t.
-*)
-
-Lemma empty_subst_on_term:
- forall (t : term),
+Lemma empty_subst_on_term: forall (t : term),
   apply_subst t [] == t.
 Proof.
- intros. induction t.
- - reflexivity.
- - simpl. reflexivity.
- - simpl. reflexivity.
- - simpl. rewrite IHt1. rewrite IHt2. reflexivity.
- - simpl. rewrite IHt1. rewrite IHt2. reflexivity.
+  intros. induction t.
+  - reflexivity.
+  - simpl. reflexivity.
+  - simpl. reflexivity.
+  - simpl. rewrite IHt1. rewrite IHt2. reflexivity.
+  - simpl. rewrite IHt1. rewrite IHt2. reflexivity.
 Qed.
 
-(** This another intutive helper lemma that states that if the empty substitution is applied on any term t, and the
-resulting term is equivalent to the ground term T0, then the input term t must be equivalent to the ground term T0.
-*)
+(** This another intutive helper lemma that states that if the empty
+    substitution is applied on any term _t_, and the resulting term is
+    equivalent to the ground term [T0], then the input term _t_ must be
+    equivalent to the ground term [T0]. *)
 
-Lemma app_subst_T0:
- forall (t : term),
+Lemma app_subst_T0: forall (t : term),
  apply_subst t [] == T0 -> t == T0.
 Proof.
-intros. rewrite empty_subst_on_term in H. apply H.
+  intros. rewrite empty_subst_on_term in H. apply H.
 Qed.
 
-(** This is another intutitve lemma that uses classical logic for it proof. It states that any term t, can be equivalent to the ground term
-T0 or it cannot be equivalent to it.
-*)
+(** This is another intutitve lemma that uses classical logic for it proof. It
+    states that any term _t_, can be equivalent to the ground term [T]0 or it
+    cannot be equivalent to it. *)
 
-Lemma T0_or_not_T0:
- forall (t : term),
- t == T0 \/ ~ (t == T0).
+Lemma T0_or_not_T0: forall (t : term),
+ t == T0 \/ ~ t == T0.
 Proof.
- intros. pose proof classic. specialize (H (t == T0)). apply H.
+  intros. pose proof classic. specialize (H (t == T0)). apply H.
 Qed.
 
-(** This is another intuitive helper lemma that states: if applying a substitution sig on a term t gives a term equivalent to T0
-then there exists a substitution that applying it to term t gives a term equivalent to T0.
-*)
+(** This is another intuitive helper lemma that states: if applying a
+    substitution $\sigma$ on a term _t_ gives a term equivalent to [T0] then
+    there exists a substitution that applying it to term _t_ gives a term
+    equivalent to [T0] (which is obvious since we already know $\sigma$ exists
+    for that task). *)
 
-Lemma exists_subst:
- forall (t : term) (sig : subst),
- apply_subst t sig == T0 -> exists s, apply_subst t s == T0.
+Lemma exists_subst: forall (t : term) (sig : subst),
+  apply_subst t sig == T0 -> exists s, apply_subst t s == T0.
 Proof.
- intros. exists sig. apply H.
+  intros. exists sig. apply H.
 Qed.
 
-
-(** This is another intuitive helper lemma that states: if applying a substitution sig on a term t gives a term equivalent to T0
-then there exists a substitution that applying it to term t gives a term equivalent to T0 (which is obvious since we already know sig exists
-for that task.
-*)
-
-Lemma t_id_eqv :
- forall (t : term),
- t == t.
+Lemma t_id_eqv : forall (t : term),
+  t == t.
 Proof.
- intros. reflexivity.
+  intros. reflexivity.
 Qed.
 
-(**  This a helper lemma that states : if two subst options (specifically Some subst) are equal then the subst (substitutions) 
-contained within the Some subst option are also equal.
-*)
+(** This a helper lemma that states: if two [options subst]s (specifically
+    [Some]) are equal then the substitutions contained within the [option subst]
+    are also equal. *)
 
 Lemma eq_some_eq_subst (s1 s2: subst) :
-  (Some s1 = Some s2) -> s1 = s2.
+  Some s1 = Some s2 -> s1 = s2.
 Proof.
-  intros.   congruence.
+  intros. congruence.
 Qed.
 
-(**  This a helper lemma that states : if the find_unifier function (the one that tries to find a ground unifier for term t) does not find a unifier (returns None subst) for an input term t
-then it not True (true not in "boolean format" but as a Proposition) that the find_unifier function produces a Some subst.
-This lemma and the following ones that are similar, are very useful for the intermediate proofs because we are able to convert
-a Proposition about the return type of the find_unifier function to an equivalent one, e.g. from None subst to Some subst and vice versa.
-*)
+(** This a helper lemma that states: if the [find_unifier] function (the one
+    that tries to find a ground unifier for term _t_) does not find a unifier
+    (returns [None]) for an input term _t_ then it not [True] (true not in
+    "boolean format" but as a proposition) that the [find_unifier] function
+    produces a [Some subst]. This lemma and the following ones that are similar,
+    are very useful for the intermediate proofs because we are able to convert a
+    proposition about the return type of the [find_unifier] function to an
+    equivalent one, e.g. from [None subst] to [Some subst] and vice versa. *)
 
 Lemma None_is_not_Some (t: term):
-  (find_unifier t) = None -> (forall (sig: subst), ~ (find_unifier t) = Some sig).
+  find_unifier t = None ->
+  forall (sig: subst), ~ find_unifier t = Some sig.
 Proof.
-  intros.
-  congruence.
+  intros. congruence.
 Qed.
 
-(**  This a helper lemma similar to the previous one that states : if the find_unifier function (the one that tries to find a ground unifier 
-for term t) finds a unifier (returns Some subst) for an input term t
-then it is not True (true not in "boolean format" but as a Proposition) that the find_unifier function produces a None subst.
-*)
+(** This a helper lemma similar to the previous one that states: if the
+    [find_unifier] function (the one that tries to find a ground unifier for
+    term _t_) finds a unifier (returns $Some \sigma$) for an input term _t_ then
+    it is not [True] (true not in "boolean format" but as a proposition) that
+    the [find_unifier] function produces a [None subst]. *)
 
 Lemma Some_is_not_None (sig: subst) (t: term):
-  (find_unifier t) = Some sig -> ~ (find_unifier t = None).
+  find_unifier t = Some sig -> ~ find_unifier t = None.
 Proof.
-  intros.
-  congruence.
+  intros. congruence.
 Qed.
 
-(**  This a helper lemma similar to the previous ones that states : if the find_unifier function (the one that tries to find a ground unifier 
-for term t) does not find a unifier that returns None subst for an input term t
-then it is True (true not in "boolean format" but as a Proposition) that the find_unifier function produces a Some subst.
-*)
+(** This a helper lemma similar to the previous ones that states: if the
+    [find_unifier] function (the one that tries to find a ground unifier for
+    term _t_) does not find a unifier that returns [None] for an input term _t_
+    then it is [True] (true not in "boolean format" but as a proposition) that
+    the [find_unifier] function produces a [Some subst]. *)
 
 Lemma not_None_is_Some (t: term) :
-  ~ (find_unifier t = None) -> exists sig : subst, (find_unifier t) = Some sig.
+  ~ find_unifier t = None ->
+  exists sig : subst, find_unifier t = Some sig.
 Proof.
   intros H.
   destruct (find_unifier t) as [ti | ].
@@ -699,110 +683,109 @@ Proof.
   - congruence.
 Qed.
 
-(** This is an intutitive helper lemma that uses classical logic to prove the validity of an alternate 
-version of the contrapositive proposition: 
-if p then q -> not q then not p, but with each entity (proposition q or p) negated.
-*)
+(** This is an intutitive helper lemma that uses classical logic to prove the
+    validity of an alternate version of the contrapositive proposition: if [p]
+    then [q] implies if not [q] then not [p], but with each entity (proposition
+    [q] and [p]) negated. *)
 
-Lemma contrapositive_opposite :
-  forall p q,  (~p -> ~q) -> q ->p.
+Lemma contrapositive_opposite : forall p q,
+  (~p -> ~q) ->
+  q -> p.
 Proof.
-  intros.
-  apply NNPP. firstorder.
+  intros. apply NNPP. firstorder.
 Qed.
 
-(** This is an intutitive helper lemma that uses classical logic to prove the validity of the contrapositive proposition: 
-if p then q -> not q then not p .
-*)
+(** This is an intutitive helper lemma that uses classical logic to prove the
+    validity of the contrapositive proposition: if [p] then [q] implies not [q]
+    then not [p]. *)
 
-Lemma contrapositive :
-forall (p q : Prop),  (p -> q) -> ( ~q -> ~p).
+Lemma contrapositive : forall (p q : Prop),
+  (p -> q) ->
+  (~q -> ~p).
+Proof.
+  intros. firstorder.
+Qed.
+
+
+(** ** Intermediate Lemmas *)
+
+(** In this subsection we prove a series of lemmas for each of the two
+    statements of the final proof, which were: 1) if a term is unifiable, then
+    [Lowenheim_Main] function produces a most general unifier (mgu). 2) if a
+    term is not unifiable, then [Lownheim_Main] function produces a [None]
+    substitution. *)
+
+
+(** *** [None] Substitution Case *)
+
+(** In this secton we prove intermediate lemmas useful for the second statement
+    of the final proof: if a term is not unifiable, then [Lownheim_Main]
+    function produces a [None] substitution. *)
+
+
+(** Lemma to show that if [find_unifier] returns [Some subst], the term is
+    unifiable. *)
+
+Lemma some_subst_unifiable: forall (t : term),
+  (exists sig, find_unifier t = Some sig) ->
+  unifiable t.
 Proof.
   intros.
-  firstorder.
-Qed.
-  
-
-
-
-
-
-(** ** Intermediate lemmas   *)
-
-(** In this sub-section we prove a series of lemmas for each of the two statements of the final proof, which were:
-      1) if a term is unifiable, then Lowenheim_Main function produces a most general unifier (mgu).
-      2) if a term is not unifiable, then Lownheim_Main function produces a None substitution.
-
-*)
-
-
-
-(** *** None subst case *)
-
-(** In this sector we prove intermediate lemmas usefule for the second statement of the final proof:
-     if a term is not unifiable, then Lownheim_Main function produces a None substitution.
-*)
-
-
-
-(** Lemma to show that if find unifier returns Some subst, the term is unifiable 
-*)
-
-Lemma some_subst_unifiable:
- forall (t : term),
-  (exists sig, (find_unifier t) = Some sig) -> (unifiable t).
-Proof.
- intros.
- destruct H as [sig1 H1].
- induction t.
- -  unfold unifiable . exists []. unfold unifier. simpl. reflexivity.
- - simpl in H1. inversion H1.
- - unfold unifiable. exists sig1. unfold find_unifier in H1.
-    remember (update_term (VAR v) (rec_subst (VAR v) (term_unique_vars (VAR v)) [])) in H1.
+  destruct H as [sig1 H1].
+  induction t.
+  - unfold unifiable. exists []. unfold unifier. simpl. reflexivity.
+  - simpl in H1. inversion H1.
+  - unfold unifiable. exists sig1. unfold find_unifier in H1.
+    remember (update_term (VAR v) (rec_subst (VAR v)
+      (term_unique_vars (VAR v)) [])) in H1.
     destruct t.
     + unfold update_term in Heqt. pose proof simplify_eqv.
-      specialize (H (apply_subst (VAR v) (rec_subst (VAR v) (term_unique_vars (VAR v)) []))).
-       symmetry in Heqt. apply eq_some_eq_subst in H1.
-      rewrite H1 in H. rewrite H1 in Heqt. 
-     rewrite Heqt in H. symmetry in H. apply H.
+      specialize (H (apply_subst (VAR v) (rec_subst (VAR v)
+        (term_unique_vars (VAR v)) []))).
+      symmetry in Heqt. apply eq_some_eq_subst in H1.
+      rewrite H1 in H. rewrite H1 in Heqt.
+      rewrite Heqt in H. symmetry in H. apply H.
     + simpl in H1. inversion H1.
     + inversion H1.
     + inversion H1.
     + inversion H1.
- - unfold unifiable. exists sig1. unfold find_unifier in H1.
-   remember (update_term (t1 + t2) (rec_subst (t1 + t2) (term_unique_vars (t1 + t2)) [])) in H1.
-  destruct t.
-  + unfold update_term in Heqt. pose proof simplify_eqv.
-    specialize (H (apply_subst (t1 + t2) (rec_subst (t1 + t2) (term_unique_vars (t1 + t2)) []))).
-       symmetry in Heqt. apply eq_some_eq_subst in H1.
-      rewrite H1 in H. rewrite H1 in Heqt. 
-     rewrite Heqt in H. symmetry in H. apply H.
-   + inversion H1.
-   + inversion H1.
-   + inversion H1.
-   + inversion H1.
- -  unfold unifiable. exists sig1. unfold find_unifier in H1.
-   remember (update_term (t1 * t2) (rec_subst (t1 * t2) (term_unique_vars (t1 * t2)) [])) in H1.
-  destruct t.
-  + unfold update_term in Heqt. pose proof simplify_eqv.
-    specialize (H (apply_subst (t1 * t2) (rec_subst (t1 * t2) (term_unique_vars (t1 * t2)) []))).
-       symmetry in Heqt. apply eq_some_eq_subst in H1.
-      rewrite H1 in H. rewrite H1 in Heqt. 
-     rewrite Heqt in H. symmetry in H. apply H.
-   + inversion H1.
-   + inversion H1.
-   + inversion H1.
-   + inversion H1.
+  - unfold unifiable. exists sig1. unfold find_unifier in H1.
+    remember (update_term (t1 + t2) (rec_subst (t1 + t2)
+      (term_unique_vars (t1 + t2)) [])) in H1.
+    destruct t.
+    + unfold update_term in Heqt. pose proof simplify_eqv.
+      specialize (H (apply_subst (t1 + t2) (rec_subst (t1 + t2)
+        (term_unique_vars (t1 + t2)) []))).
+      symmetry in Heqt. apply eq_some_eq_subst in H1.
+      rewrite H1 in H. rewrite H1 in Heqt.
+      rewrite Heqt in H. symmetry in H. apply H.
+    + inversion H1.
+    + inversion H1.
+    + inversion H1.
+    + inversion H1.
+  - unfold unifiable. exists sig1. unfold find_unifier in H1.
+    remember (update_term (t1 * t2) (rec_subst (t1 * t2)
+      (term_unique_vars (t1 * t2)) [])) in H1.
+    destruct t.
+    + unfold update_term in Heqt. pose proof simplify_eqv.
+      specialize (H (apply_subst (t1 * t2) (rec_subst (t1 * t2)
+        (term_unique_vars (t1 * t2)) []))).
+      symmetry in Heqt. apply eq_some_eq_subst in H1.
+      rewrite H1 in H. rewrite H1 in Heqt.
+      rewrite Heqt in H. symmetry in H. apply H.
+    + inversion H1.
+    + inversion H1.
+    + inversion H1.
+    + inversion H1.
 Qed.
 
 
-
-
-(** Lemma to show that if no subst makes find_unifier to return Some subst, the it returns None susbt 
-*)
+(** This lemma shows that if no substituion makes [find_unifier] to return
+    [Some subst], the it returns [None]. *)
 
 Lemma not_Some_is_None (t: term) :
- ( ~ exists (sig : subst), (find_unifier t) = Some sig) -> (find_unifier t) = None.
+  ~ (exists sig, find_unifier t = Some sig) ->
+  find_unifier t = None.
 Proof.
   apply contrapositive_opposite.
   intros H.
@@ -811,210 +794,207 @@ Proof.
 Qed.
 
 
-(* Lemma to show that if a term t is not unifiable, the find_unifier function returns None subst with
-t as input
-*)
+(* Lemma to show that if a term _t_ is not unifiable, the [find_unifier]
+    function returns [None] with _t_ as input. *)
 
-Lemma not_unifiable_find_unifier_none_subst :
-forall (t : term),
-   ~ (unifiable t) -> (find_unifier t) = None.
+Lemma not_unifiable_find_unifier_none_subst : forall (t : term),
+  ~ unifiable t -> find_unifier t = None.
 Proof.
-intros.
- pose proof some_subst_unifiable.
- specialize (H0 t).
- pose proof contrapositive.
- specialize (H1 ((exists sig : subst, find_unifier t = Some sig)) ((unifiable t))).
- specialize (H1 H0). specialize (H1 H).
- pose proof not_Some_is_None.
- specialize (H2 t H1).
- apply H2.
+  intros.
+  pose proof some_subst_unifiable.
+  specialize (H0 t).
+  pose proof contrapositive.
+  specialize (H1 (exists sig : subst, find_unifier t = Some sig) (unifiable t)).
+  specialize (H1 H0). specialize (H1 H).
+  pose proof not_Some_is_None.
+  specialize (H2 t H1).
+  apply H2.
 Qed.
 
 
+(** *** [Some] Substituion Case *)
 
-(** *** Some subst case  *)
+(** In this secton we prove intermediate lemmas useful for the first statement
+    of the final proof: if a term is unifiable, then [Lowenheim_Main] function
+    produces a most general unifier (mgu). *)
 
-(** In this sector we prove intermediate lemmas usefule for the first statement of the final proof:
-     if a term is unifiable, then Lowenheim_Main function produces a most general unifier (mgu).
-*)
+(** Lemma to show that if [find_unifier] on an input term _t_ returns
+    $Some \sigma$, then $\sigma$ is a unifier of _t_. *)
 
-
-(** Lemma to show that if find_unifier on an input term t returns Some subst,
-then that subst containtes withint the option is a unifier of t. 
-*)
-
-Lemma Some_subst_unifiable :
-forall (t : term) (sig : subst),
-   (find_unifier t) = Some sig -> (unifier t sig).
+Lemma Some_subst_unifiable : forall (t : term) (sig : subst),
+  find_unifier t = Some sig -> unifier t sig.
 Proof.
-intros.
- induction t.
- - simpl in H. apply eq_some_eq_subst in H. symmetry in H. rewrite H.
-  unfold unifier. simpl. reflexivity.
- - simpl in H. inversion H.
- - unfold find_unifier in H. remember (update_term (VAR v) (rec_subst (VAR v) (term_unique_vars (VAR v)) [])) in H.
+  intros.
+  induction t.
+  - simpl in H. apply eq_some_eq_subst in H. symmetry in H. rewrite H.
+    unfold unifier. simpl. reflexivity.
+  - simpl in H. inversion H.
+  - unfold find_unifier in H. remember (update_term (VAR v)
+      (rec_subst (VAR v) (term_unique_vars (VAR v)) [])) in H.
     destruct t.
-  + unfold update_term in Heqt. pose proof simplify_eqv.
-      specialize (H0 (apply_subst (VAR v) (rec_subst (VAR v) (term_unique_vars (VAR v)) []))).
-         symmetry in Heqt. apply eq_some_eq_subst in H.
-      rewrite H in H0. rewrite H in Heqt. 
-     rewrite Heqt in H0. symmetry in H0. apply H0.
-  + inversion H.
-  + inversion H.
-  + inversion H.
-  + inversion H.
- - unfold find_unifier in H. remember (update_term (t1 + t2) (rec_subst (t1 + t2) (term_unique_vars (t1 + t2)) [])) in H.
+    + unfold update_term in Heqt. pose proof simplify_eqv.
+      specialize (H0 (apply_subst (VAR v) (rec_subst (VAR v)
+        (term_unique_vars (VAR v)) []))).
+      symmetry in Heqt. apply eq_some_eq_subst in H.
+      rewrite H in H0. rewrite H in Heqt.
+      rewrite Heqt in H0. symmetry in H0. apply H0.
+    + inversion H.
+    + inversion H.
+    + inversion H.
+    + inversion H.
+  - unfold find_unifier in H. remember (update_term (t1 + t2)
+      (rec_subst (t1 + t2) (term_unique_vars (t1 + t2)) [])) in H.
     destruct t.
-  + unfold update_term in Heqt. pose proof simplify_eqv.
-      specialize (H0 (apply_subst (t1 + t2) (rec_subst (t1 + t2) (term_unique_vars (t1 + t2)) []))).
-       symmetry in Heqt. apply eq_some_eq_subst in H.
-      rewrite H in H0. rewrite H in Heqt. 
-     rewrite Heqt in H0. symmetry in H0. apply H0.
-  + inversion H.
-  + inversion H.
-  + inversion H.
-  + inversion H.
- - unfold find_unifier in H. remember (update_term (t1 * t2) (rec_subst (t1 * t2) (term_unique_vars (t1 * t2)) [])) in H.
+    + unfold update_term in Heqt. pose proof simplify_eqv.
+      specialize (H0 (apply_subst (t1 + t2) (rec_subst (t1 + t2)
+        (term_unique_vars (t1 + t2)) []))).
+      symmetry in Heqt. apply eq_some_eq_subst in H.
+      rewrite H in H0. rewrite H in Heqt.
+      rewrite Heqt in H0. symmetry in H0. apply H0.
+    + inversion H.
+    + inversion H.
+    + inversion H.
+    + inversion H.
+  - unfold find_unifier in H. remember (update_term (t1 * t2)
+      (rec_subst (t1 * t2) (term_unique_vars (t1 * t2)) [])) in H.
     destruct t.
-  + unfold update_term in Heqt. pose proof simplify_eqv.
-      specialize (H0 (apply_subst (t1 * t2) (rec_subst (t1 * t2) (term_unique_vars (t1 * t2)) []))).
-       symmetry in Heqt. apply eq_some_eq_subst in H.
-      rewrite H in H0. rewrite H in Heqt. 
-     rewrite Heqt in H0. symmetry in H0. apply H0.
-  + inversion H.
-  + inversion H.
-  + inversion H.
-  + inversion H.
+    + unfold update_term in Heqt. pose proof simplify_eqv.
+      specialize (H0 (apply_subst (t1 * t2) (rec_subst (t1 * t2)
+        (term_unique_vars (t1 * t2)) []))).
+      symmetry in Heqt. apply eq_some_eq_subst in H.
+      rewrite H in H0. rewrite H in Heqt.
+      rewrite Heqt in H0. symmetry in H0. apply H0.
+    + inversion H.
+    + inversion H.
+    + inversion H.
+    + inversion H.
 Qed.
 
 
-(** Lemma to show that if there is a unifier, then there is a 'ground unifier'.
-*)
+(** This lemma shows that if there is a unifier, then there is a "ground
+    unifier". *)
 
-Lemma unif_some_subst :
- forall (t: term),
- (exists sig1, (unifier t sig1)) ->
- (exists sig2, (find_unifier t) = Some sig2).
+Lemma unif_some_subst : forall (t: term),
+  (exists sig1, unifier t sig1) ->
+  exists sig2, find_unifier t = Some sig2.
 Proof.
- intros.
- destruct H as [sig1 H].
+  intros.
+  destruct H as [sig1 H].
 Admitted.
 
 
-(** Lemma to show that if no subst makes find_unifier to return Some subst, the it returns None susbt 
-*)
+(** Lemma to show that if no substituion makes [find_unifier] return
+    $Some \sigma$, then it returns [None]. *)
 
 Lemma not_Some_not_unifiable (t: term) :
- ( ~ exists (sig : subst), (find_unifier t) = Some sig) -> ~ (unifiable t).
+  (~ exists sig, find_unifier t = Some sig) ->
+  ~ unifiable t.
 Proof.
- intros.
- pose proof not_Some_is_None.
- specialize (H0 t H).
- unfold unifiable.
- intro.
+  intros.
+  pose proof not_Some_is_None.
+  specialize (H0 t H).
+  unfold unifiable.
+  intro.
   unfold not in H.
- pose proof unif_some_subst.
- specialize (H2 t H1).
- specialize (H H2).
- apply H.
+  pose proof unif_some_subst.
+  specialize (H2 t H1).
+  specialize (H H2).
+  apply H.
 Qed.
- 
 
 
+(** This lemma shows that if a term is unifiable then [find_unifier] returns
+    $Some \sigma$. *)
 
-(** Lemma to show that if a term is unifiable then find_unifier returns Some subst 
-*)
-
-Lemma unifiable_find_unifier_some_subst :
-forall (t : term),
-   (unifiable t) -> (exists (sig : subst), (find_unifier t) = Some sig).
+Lemma unifiable_find_unifier_some_subst : forall (t : term),
+  unifiable t ->
+  (exists sig, find_unifier t = Some sig).
 Proof.
-intros. 
- pose proof contrapositive.
- specialize (H0 ( ~ exists (sig : subst), (find_unifier t) = Some sig) (~ (unifiable t))).
- pose proof not_Some_not_unifiable.
- specialize (H1 t). specialize (H0 H1). apply NNPP in H0.
- -  apply H0.
- -  firstorder.
+  intros.
+  pose proof contrapositive.
+  specialize (H0 (~ exists sig, find_unifier t = Some sig) (~ unifiable t)).
+  pose proof not_Some_not_unifiable.
+  specialize (H1 t). specialize (H0 H1). apply NNPP in H0.
+  - apply H0.
+  - firstorder.
 Qed.
 
 
 
-(** Lemma to show that if a term is unifiable, then find_unifier returns a unifier 
-*)
+(** This lemma shows that if a term is unifiable, then [find_unifier] returns a
+    unifier. *)
 
-Lemma find_unifier_is_unifier:
- forall (t : term),
-  (unifiable t) -> (unifier t (convert_to_subst (find_unifier t))).
+Lemma find_unifier_is_unifier: forall (t : term),
+  unifiable t -> unifier t (convert_to_subst (find_unifier t)).
 Proof.
-intros. 
- pose proof unifiable_find_unifier_some_subst.
- specialize (H0 t H).
- unfold unifier. unfold unifiable in H. simpl. unfold convert_to_subst.
- 
- destruct H0 as [sig H0]. rewrite H0. 
- pose proof Some_subst_unifiable.
- specialize (H1 t sig). specialize (H1 H0).
- unfold unifier in H1.
- apply H1.
+  intros.
+  pose proof unifiable_find_unifier_some_subst.
+  specialize (H0 t H).
+  unfold unifier. unfold unifiable in H. simpl. unfold convert_to_subst.
+  destruct H0 as [sig H0]. rewrite H0.
+  pose proof Some_subst_unifiable.
+  specialize (H1 t sig). specialize (H1 H0).
+  unfold unifier in H1.
+  apply H1.
 Qed.
 
 
 
+(** ** Gluing Everything Together For the Final Proof *)
 
-(** ** Gluing everything together for the final proof *)
+(** In this subsection we prove the two top-level final proof lemmas. Both of
+    these proofs use the intermediate lemmas proved in the previous subsections.
+    *)
 
-(** In this sub-section we prove the two top-level final proof lemmas. Both of these proofs use the intermediate lemmas proved
-in the previous subs-section
-*)
+(** The first one states that given a uniable term _t_ and the fact that our
+    Lowenheim builder produces an mgu, then the [Lowenheim_Main] function
+    also produces an mgu. *)
 
-
-(**
-The first one states that given a uniable term t and
-the fact that our lowenheim builder produces an mgu, then the Lowenheim Main function also produces an mgu.
-*)
-
-Lemma builder_to_main:
- forall (t : term),
-(unifiable t) -> most_general_unifier t (build_lowenheim_subst t (convert_to_subst (find_unifier t))) ->
- most_general_unifier t (convert_to_subst (Lowenheim_Main t)) .
+Lemma builder_to_main: forall (t : term),
+  unifiable t ->
+  most_general_unifier t (build_lowenheim_subst
+                           t (convert_to_subst (find_unifier t))) ->
+  most_general_unifier t (convert_to_subst (Lowenheim_Main t)).
 Proof.
-intros. 
-pose proof lowenheim_most_general_unifier as H1. pose proof find_unifier_is_unifier as H2.
-specialize (H2 t H). specialize (H1 t (convert_to_subst (find_unifier t))). 
-specialize (H1 H2). unfold Lowenheim_Main. destruct (find_unifier t).
- - simpl. simpl in H1. apply H1.
- - simpl in H2. unfold unifier in H2. apply app_subst_T0 in H2. simpl. 
-   repeat simpl in H1. pose proof most_general_unifier_compat. 
-   specialize (H3 t T0 H2). specialize (H3 []).
-   rewrite H3. unfold most_general_unifier. intros. 
-   unfold more_general_substitution. exists s'. unfold substitution_composition. 
-   intros. simpl. reflexivity. 
+  intros.
+  pose proof lowenheim_most_general_unifier as H1.
+  pose proof find_unifier_is_unifier as H2.
+  specialize (H2 t H). specialize (H1 t (convert_to_subst (find_unifier t))).
+  specialize (H1 H2). unfold Lowenheim_Main. destruct (find_unifier t).
+  - simpl. simpl in H1. apply H1.
+  - simpl in H2. unfold unifier in H2. apply app_subst_T0 in H2. simpl.
+    repeat simpl in H1. pose proof most_general_unifier_compat.
+    specialize (H3 t T0 H2). specialize (H3 []).
+    rewrite H3. unfold most_general_unifier. intros.
+    unfold more_general_substitution. exists s'.
+    unfold substitution_composition.
+    intros. simpl. reflexivity.
 Qed.
 
 
-(**
-This the final top-level lemma that encapsulates all our efforts so far. It proves the two main statements required for the final
-proof. The two statements, as phrased in the beggining of the chapter are:
-      1) if a term is unifiable, then our own defined Lowenheim_Main function produces a most general unifier (mgu).
-      2) if a term is not unifiable, then our own defined Lownheim_Main function produces a None substitution.
-The two Propositions are related with the "/\" symbol (namely, the Propositional "and") and each is proven seperately using the 
-intermediate lemmas proved above. This is why the final top-level proof is relatively short, because a lot of the singnificant
-components of the proof have already been proven as intermediate lemmas.
-*)
+(** This the final top-level lemma that encapsulates all our efforts so far. It
+    proves the two main statements required for the final proof. The two
+    statements, as phrased in the beginning of the chapter are: 1) if a term is
+    unifiable, then our own defined [Lowenheim_Main] function produces a most
+    general unifier (mgu). 2) if a term is not unifiable, then our own defined
+    [Lownheim_Main] function produces a [None] substitution. The two
+    propositions are related with the "$\wedge$" symbol (namely, the
+    propositional "and") and each is proven seperately using the intermediate
+    lemmas proven above. This is why the final top-level proof is relatively
+    short, because a lot of the significant components of the proof have already
+    been proven as intermediate lemmas. *)
 
-Lemma lowenheim_main_most_general_unifier:
- forall (t: term),
- ((unifiable t) -> most_general_unifier t (convert_to_subst (Lowenheim_Main t)))
- /\ 
- (~(unifiable t) -> (Lowenheim_Main t) = None ).
+Lemma lowenheim_main_most_general_unifier: forall (t: term),
+ (unifiable t -> most_general_unifier t (convert_to_subst (Lowenheim_Main t)))
+ /\
+ (~ unifiable t -> Lowenheim_Main t = None).
 Proof.
- intros. 
- split. 
- - intros. apply builder_to_main.
-  +  apply H.
-  + apply lowenheim_most_general_unifier. apply find_unifier_is_unifier. apply H.
- - intros. pose proof not_unifiable_find_unifier_none_subst. 
-   specialize (H0 t H). unfold Lowenheim_Main. rewrite H0. reflexivity.
+  intros.
+  split.
+  - intros. apply builder_to_main.
+    + apply H.
+    + apply lowenheim_most_general_unifier. apply find_unifier_is_unifier.
+      apply H.
+  - intros. pose proof not_unifiable_find_unifier_none_subst.
+    specialize (H0 t H). unfold Lowenheim_Main. rewrite H0. reflexivity.
 Qed.
-
